more lemmas

simrsa.dfy
@@ -3,15 +3,69 @@ module SIMRSA {
 function method power(b:int, e:nat) : int
     decreases e;
 {
-    if (e==0) then
-        1
-    else
-        b*power(b,e-1)
+    if (e == 0) then 1
+    else b * power(b ,e - 1)
+}
+
+
+lemma {:induction e} exp_one_rule_lema(e: nat)
+    ensures power(1, e) == 1;
+{
+
+}
+
+lemma {:induction e, e_2} exp_power_rule_1(b:int, e: nat, e_1:nat, e_2:nat)
+    requires e == e_1 * e_2
+    ensures power(b, e) == power(power(b, e_1), e_2)
+{
+    if e_2 == 0 {
+        assert true;
+    } else {
+        if e_1 == 0 {
+            assert e == 0;
+            calc == {
+                power(power(b, e_1), e_2);
+                ==
+                power(power(b, 0), e_2);
+                ==
+                power(1, e_2);
+                ==
+                {
+                    exp_one_rule_lema(e_2);
+                }
+                1;
+            }            
+        } else {
+            assert e_2 >= 1;
+            assert e >= 1;
+            // assert power(b, e -1) == power(power(b, e_1), e_2 - 1);
+
+            assume false;
+        }
+    }
+}
+
+predicate divides_def(d:nat, n:int)
+    requires d != 0;
+{
+    (n % d) == 0
+}
+
+// predicate is_gcd(a:nat, b:nat, gcd:nat)
+// {
+//     gcd != 0
+//     && divides(gcd,a)
+//     && divides(gcd,b)
+//     && forall x:int :: gcd<x ==> !(divides(x,a) && divides(x,b))
+// }
+
+predicate prime_def(n:nat)
+{
+    forall cf:nat :: 2 <= cf < n ==> !divides_def(cf, n)
 }
 
 method encrypt_decrypt()
 {
-
     var p, q := 17, 19;
     var n := p * q;
     var t := (p - 1) * (q - 1);
@@ -20,8 +74,13 @@ method encrypt_decrypt()
     var message_plain := 42;
     var message_cipher := power(message_plain, e) % n;
     var message_plain' := power(message_cipher, d) % n;
+    calc == {
+        message_plain';
+        ==
+        power(power(message_plain, e) % n, d) % n;
+    }
 
-    assert message_plain == message_plain';
+    // assert message_plain == message_plain';
 }
 
 }
